Alternative heap-sort approach, mostly verified
Switch out the standard heap-sort, in which the heap points in the opposite
direction, for a list-of-heaps sort in which power-of-two-minus-one sized heaps
point in the correct direction within the array. This has the advantage that an
already sorted array is confirmed sorted without moving anything and in linear
time. It also "agrees" with the functional model.

Problem though, the mapping of the multiple heaps into the array gets painful
to reason about. Saving before trying a different approach.

basis/heap_sort_monadicScript.sml
@@ -10,6 +10,8 @@ Ancestors
 Libs
   preamble ml_translatorLib ml_monad_translator_interfaceLib
 
+val _ = ParseExtras.tight_equality();
+
 (* Part 1. Translator Setup. *)
 
 (* Set up translator to not check subtractions never underflow. *)
@@ -20,12 +22,13 @@ val _ = set_up_monadic_translator ();
 (* The type variable used as parameter to the state type. It seems very
    important that this is used consistently. Strangely `'a` seems to work (for
    the current code) though it created problems in a previous iteration. *)
-val tvar = ``: 'a``;
+val tvar = ``: 'state``;
 
 (* Create the data type to handle the references *)
 Datatype:
   state_refs = <|
                  heap_array : ( ^tvar ) list;
+                 sz_array : num list;
                 |>
 End
 
@@ -40,10 +43,13 @@ val config = local_state_config |>
               with_state state_type |>
               with_exception ``:state_exn`` |>
               with_resizeable_arrays [
-                ("heap_array", listSyntax.mk_list ([], tvar), ``Subscript``, ``Subscript``)
+                ("heap_array", listSyntax.mk_list ([], tvar), ``Subscript``, ``Subscript``),
+                ("sz_array", ``[] : num list``, ``Subscript``, ``Subscript``)
               ];
 
 val _ = start_translation config;
+
+val run_init_state_def = define_run state_type [] "init_state";
 
 (* Part 2. Define monadic variants of functions from heap_sort_in_fun theory. *)
 
@@ -315,8 +321,6 @@ QED
 
 (* Part 3. Translation into CakeML AST. *)
 
-val run_init_state_def = define_run state_type [] "init_state";
-
 Definition heap_sort_via_monad_aux1_def:
   heap_sort_via_monad_aux1 R x xs =
   (do
@@ -407,4 +411,1158 @@ val heap_sort_via_monad_aux2_v_thm = heap_sort_via_monad_aux2_def
 
 val heap_sort_via_monad_v_thm = heap_sort_via_monad_def |> translate;
 
+
+(* Second variant. *)
+(* Heap list version. *)
+
+(* 'start_translation' parts at the top *)
+
+(* Positions of the left child in a suffix encoded balanced tree
+   of height ht. *)
+Definition sfx_heap_left_def:
+  sfx_heap_left i ht = (i - (2 EXP (ht - 1)))
+End
+
+(* Insert a value into a balanced suffix heap of height ht, replacing the
+   current top element which is at index i. *)
+Definition insert_into_sfx_heap_def:
+  insert_into_sfx_heap R i ht x = if ht <= 1
+  then update_heap_array i x
+  else do
+    l <- return (sfx_heap_left i ht);
+    r <- return (i - 1);
+    lx <- heap_array_sub l;
+    rx <- heap_array_sub r;
+    if R lx x /\ R rx x
+    then update_heap_array i x
+    else if R lx rx
+    then do
+      update_heap_array i rx;
+      insert_into_sfx_heap R r (ht - 1) x
+    od
+    else do
+      update_heap_array i lx;
+      insert_into_sfx_heap R l (ht - 1) x
+    od
+  od
+End
+
+(* Insert a value into a sequence of balanced suffix heaps, heights stored
+   in positions [0 ..< j] of the sz_array. Replace the top elements of the
+   final heap, which is at index i.  *)
+Definition insert_into_sfx_heap_list_def:
+  insert_into_sfx_heap_list R i j x =
+  if j <= 1 then do
+    ht <- sz_array_sub (j - 1);
+    insert_into_sfx_heap R i ht x
+  od
+  else do
+    ht <- sz_array_sub (j - 1);
+    i2 <- return ((i + 1) - (2 EXP ht));
+    t2x <- heap_array_sub i2;
+    cond1 <- return (~ R t2x x);
+    cond <- if cond1 /\ (1 < ht)
+      then do
+        l <- return (sfx_heap_left i ht);
+        r <- return (i - 1);
+        lx <- heap_array_sub l;
+        rx <- heap_array_sub r;
+        return (~ R t2x lx /\ ~ R t2x rx)
+      od
+      else return cond1;
+    if cond
+    then do
+      update_heap_array i t2x;
+      insert_into_sfx_heap_list R i2 (j - 1) x
+    od
+    else insert_into_sfx_heap R i ht x
+  od
+End
+
+(* Add another element to the final heap in a sequence of balanced suffix
+   heaps with i total elements and j total heaps. *)
+Definition add_to_sfx_heaps_step1_def:
+  add_to_sfx_heaps_step1 i j = do
+    merge <- if j <= 1
+      then return F
+      else do
+        n1 <- sz_array_sub (j - 1);
+        n2 <- sz_array_sub (j - 2);
+        return (n1 = n2);
+      od;
+    if merge
+    then do
+      n <- sz_array_sub (j - 2);
+      update_sz_array (j - 2) (n + 1);
+      return (j - 1);
+    od
+    else do
+      update_sz_array j 1;
+      return (j + 1);
+    od
+  od
+End
+
+(* Also set the top element and preserve invariants. *)
+Definition add_to_sfx_heaps_def:
+  add_to_sfx_heaps R i j x = do
+    j' <- add_to_sfx_heaps_step1 i j;
+    insert_into_sfx_heap_list R i j' x;
+    return j'
+  od
+End
+
+Definition add_all_to_sfx_heaps_def:
+  (add_all_to_sfx_heaps R i j [] = return (i, j)) /\
+  (add_all_to_sfx_heaps R i j (x :: xs) = do
+    j <- add_to_sfx_heaps R i j x;
+    add_all_to_sfx_heaps R (i + 1) j xs;
+  od)
+End
+
+Definition reinsert_tree_def:
+  reinsert_tree R i j ht =
+  do
+    update_sz_array j ht;
+    x <- heap_array_sub (i - 1);
+    upd <- if 0 < j then do
+      i2 <- return (i - (2 EXP ht));
+      t2x <- heap_array_sub i2;
+      return (~ (R t2x x))
+    od else return F;
+    if upd
+    then insert_into_sfx_heap_list R (i - 1) (j + 1) x
+    else return ();
+  od
+End
+
+Definition sfx_trees_to_list_def:
+  sfx_trees_to_list R i j acc =
+  if i = 0 then return acc
+  else do
+    ht <- sz_array_sub (j - 1);
+    x <- heap_array_sub (i - 1);
+    if ht <= 1 then sfx_trees_to_list R (i - 1) (j - 1) (x :: acc)
+    else do
+      l <- return (sfx_heap_left i ht);
+      reinsert_tree R l (j - 1) (ht - 1);
+      reinsert_tree R (i - 1) j (ht - 1);
+      sfx_trees_to_list R (i - 1) (j + 1) (x :: acc)
+    od
+  od
+End
+
+Definition sort_via_sfx_trees_worker_def:
+  sort_via_sfx_trees_worker R x xs = do
+      sz <- return (LENGTH xs);
+      alloc_heap_array sz x;
+      alloc_sz_array (LOG2 sz + 3) 0;
+      (i, j) <- add_all_to_sfx_heaps R 0 0 xs;
+      sfx_trees_to_list R i j []
+  od
+End
+
+Definition sort_via_sfx_trees_run_worker_def:
+  sort_via_sfx_trees_run_worker R x xs =
+  run_init_state (sort_via_sfx_trees_worker R x xs)
+    (init_state [] [])
+End
+
+Definition sort_via_sfx_trees_def:
+  sort_via_sfx_trees R xs = (case xs of [] => []
+    | x :: _ => (case sort_via_sfx_trees_run_worker R x xs of
+        M_success ys => ys
+      | _ => [])
+  )
+End
+
+
+(* Equivalence of second variant. *)
+
+Definition bs_tree_to_list_def:
+  (bs_tree_to_list 0 t = []) /\
+  (bs_tree_to_list (SUC ht) t =
+     bs_tree_to_list ht (case t of Node _ l r => l | _ => t) ++
+     bs_tree_to_list ht (case t of Node _ l r => r | _ => t) ++
+     [case t of Node x l r => x]
+  )
+End
+
+Theorem bs_tree_to_list_tree_rec[local]:
+  (i = 0 ==> bs_tree_to_list i Empty_Tree = []) /\
+  (0 < i ==> bs_tree_to_list i (Node x l r) =
+    bs_tree_to_list (i - 1) l ++
+    bs_tree_to_list (i - 1) r ++
+    [x])
+Proof
+  Cases_on `i` \\ simp [bs_tree_to_list_def]
+QED
+
+Definition two_exp_min_1_def:
+  two_exp_min_1 i = (2n EXP i) - 1
+End
+
+Theorem two_exp_min_1_less_rec:
+  0 < i ==> two_exp_min_1 i = two_exp_min_1 (i - 1) + two_exp_min_1 (i - 1) + 1
+Proof
+  Cases_on `i`
+  \\ fs [two_exp_min_1_def, EXP]
+  \\ rw [SUB_RIGHT_ADD]
+QED
+
+Theorem two_exp_min_1_rec:
+  two_exp_min_1 0 = 0 /\
+  two_exp_min_1 (SUC i) = two_exp_min_1 i + two_exp_min_1 i + 1
+Proof
+  simp [two_exp_min_1_less_rec] \\ simp [two_exp_min_1_def]
+QED
+
+Theorem to_two_exp_min_1:
+  (2n EXP i) = (two_exp_min_1 i + 1)
+Proof
+  rw [two_exp_min_1_def, SUB_RIGHT_ADD]
+QED
+
+Theorem sfx_heap_left_two_exp_min_1:
+  sfx_heap_left n ht = n - (two_exp_min_1 (ht - 1)) - 1
+Proof
+  simp [sfx_heap_left_def, to_two_exp_min_1]
+QED
+
+Theorem LENGTH_bs_tree_to_list:
+  ! i t. LENGTH (bs_tree_to_list i t) = two_exp_min_1 i
+Proof
+  Induct 
+  \\ simp [bs_tree_to_list_def, two_exp_min_1_rec]
+QED
+
+Definition tree_balanced_height_def:
+  (tree_balanced_height i Empty_Tree = (i = 0n)) /\
+  (tree_balanced_height i (Node x l r) = (
+    (i > 0) /\ tree_balanced_height (i - 1) l /\
+        tree_balanced_height (i - 1) r)
+  )
+End
+
+Theorem tree_balanced_height_0:
+  (tree_balanced_height 0 t = (t = Empty_Tree))
+Proof
+  Cases_on `t` \\ simp [tree_balanced_height_def]
+QED
+
+Theorem tree_balanced_height_pos:
+  0 < ht ==> tree_balanced_height ht t =
+    (?x l r. t = Node x l r /\ tree_balanced_height (ht - 1) l /\
+        tree_balanced_height (ht - 1) r)
+Proof
+  Cases_on `t` \\ simp [tree_balanced_height_def]
+QED
+
+(*
+Theorem tree_balanced_height_length_sfx_eq:
+  tree_balanced_height ht t ==>
+    (LENGTH (tree_sfx_list t) = ((2 EXP ht) - 1))
+Proof
+  qid_spec_tac `ht` \\ Induct_on `t`
+  \\ fs [tree_sfx_list_def, tree_balanced_height_def]
+  \\ rw []
+  \\ Cases_on `ht` \\ fs []
+  \\ res_tac
+  \\ simp [EXP]
+  \\ simp [SUB_RIGHT_ADD]
+  \\ rw []
+QED
+*)
+
+(*
+Theorem tree_balanced_height_length_sfx_eq:
+  tree_balanced_height ht t ==> 0 < ht ==>
+    (LENGTH (tree_sfx_list t) = two_exp_min_2 ht + 1)
+Proof
+  qid_spec_tac `ht` \\ Induct_on `t`
+  \\ simp [tree_balanced_height_def, tree_sfx_list_def, two_exp_min_2_rec]
+  \\ rw []
+  \\ Cases_on `ht` \\ fs []
+  \\ simp [two_exp_min_2_rec]
+  \\ rw []
+  \\ fs [tree_balanced_height_0, tree_sfx_list_def]
+  \\ res_tac
+  \\ simp []
+QED
+
+Definition tree_list_len_eq_def:
+  tree_list_len_eq xs t ht i =
+  (tree_balanced_height ht t /\
+    (i = LENGTH xs + LENGTH (tree_sfx_list t) - 1))
+End
+
+Theorem tree_list_len_eq_bases:
+  (tree_list_len_eq xs Empty_Tree ht i = ((ht = 0) /\ (i = LENGTH xs - 1))) /\
+  (tree_list_len_eq xs t 0 i = ((t = Empty_Tree) /\ (i = LENGTH xs - 1)))
+Proof
+  simp [tree_list_len_eq_def, tree_balanced_height_def, tree_sfx_list_def]
+  \\ Cases_on `t` \\ simp [tree_balanced_height_def, tree_sfx_list_def]
+QED
+
+Theorem tree_list_len_eq_split:
+  tree_list_len_eq xs (Node x l r) ht i ==>
+  tree_list_len_eq xs l (ht - 1) (i - (2 EXP (ht - 1))) /\
+  tree_list_len_eq (xs ++ tree_sfx_list l) r (ht - 1) (i - 1)
+Proof
+  rw [tree_list_len_eq_def]
+  \\ fs [tree_balanced_height_def, tree_sfx_list_def]
+  \\ imp_res_tac tree_balanced_height_length_sfx_eq
+  \\ Cases_on `ht` \\ full_simp_tac std_ss []
+  \\ simp [EXP]
+  \\ Cases_on `n = 0` \\ fs []
+  \\ subgoal `?x. 2 EXP n = (2 + x)`
+  \\ fs []
+  \\ qexists_tac `(2 EXP n) - 2`
+  \\ simp [SUB_RIGHT_ADD]
+  \\ rw []
+QED
+
+Definition tree_len_eq_def:
+  tree_len_eq n t ht i =
+  (tree_balanced_height ht t /\ (i = n + LENGTH (tree_sfx_list t) - 1))
+End
+
+Theorem tree_len_eq_bases:
+  (tree_len_eq n Empty_Tree ht i = ((ht = 0) /\ (i = n - 1))) /\
+  (tree_len_eq n t 0 i = ((t = Empty_Tree) /\ (i = n - 1)))
+Proof
+  simp [tree_len_eq_def, tree_balanced_height_def, tree_sfx_list_def]
+  \\ Cases_on `t` \\ simp [tree_balanced_height_def, tree_sfx_list_def]
+QED
+
+Theorem tree_len_eq_split:
+  tree_len_eq n (Node x l r) ht i ==>
+  tree_len_eq n l (ht - 1) (i - (2 EXP (ht - 1))) /\
+  tree_len_eq (n + LENGTH (tree_sfx_list l)) r (ht - 1) (i - 1)
+Proof
+  rw [tree_len_eq_def]
+  \\ fs [tree_balanced_height_def, tree_sfx_list_def]
+  \\ imp_res_tac tree_balanced_height_length_sfx_eq
+  \\ full_simp_tac std_ss []
+  \\ subgoal `ht > 1 ==> ?x. 2 EXP (ht - 1) = (2 + x)`
+  \\ Cases_on `ht - 1` \\ Cases_on `ht` \\ full_simp_tac std_ss []
+  \\ fs []
+  \\ qexists_tac `(2 EXP SUC n) - 2`
+  \\ simp [SUB_RIGHT_ADD]
+  \\ rw []
+QED
+*)
+
+Theorem return_bind_eq:
+  st_ex_bind (return v) f = f v
+Proof
+  simp [ml_monadBaseTheory.st_ex_bind_def, ml_monadBaseTheory.st_ex_return_def, FUN_EQ_THM]
+QED
+
+(*
+Theorem heap_array_sub_eq_intro:
+  tree_list_len_eq xs t ht i ==>
+  (st.heap_array = xs ++ tree_sfx_list t ++ ys) ==>
+  0 < ht ==>
+  (f (case t of Node y _ _ => y) st = (M_success v, st_fin)) ==>
+  (st_ex_bind (heap_array_sub i) f st = (M_success v, st_fin))
+Proof
+  simp [fetch "-" "heap_array_sub_def"]
+  \\ simp [ml_monadBaseTheory.monad_eqs]
+  \\ rw []
+  \\ imp_res_tac tree_balanced_height_length_sfx_eq
+  \\ simp []
+  \\ fs [tree_list_len_eq_def]
+  \\ Cases_on `t` \\ fs [tree_balanced_height_def]
+  \\ fs [tree_sfx_list_def]
+  \\ simp [EL_APPEND]
+QED
+
+Theorem heap_array_sub_eq_intro2:
+  tree_len_eq n t ht i ==>
+  0 < ht ==>
+  (DROP n st.heap_array = tree_sfx_list t ++ ys) ==>
+  (f (case t of Node y _ _ => y) st = (M_success v, st_fin)) ==>
+  (st_ex_bind (heap_array_sub i) f st = (M_success v, st_fin))
+Proof
+  simp [fetch "-" "heap_array_sub_def"]
+  \\ simp [ml_monadBaseTheory.monad_eqs]
+  \\ rpt disch_tac
+  \\ Cases_on `LENGTH st.heap_array <= n`
+  >- (
+    fs (RES_CANON miscTheory.DROP_NIL)
+    \\ Cases_on `t` \\ fs [tree_sfx_list_def, tree_len_eq_bases]
+  )
+  \\ subgoal `?xs. (st.heap_array = xs ++ tree_sfx_list t ++ ys) /\ (LENGTH xs = n)`
+  >- (
+    qexists_tac `TAKE n st.heap_array`
+    \\ simp [LENGTH_TAKE]
+    \\ metis_tac [TAKE_DROP, APPEND_ASSOC]
+  )
+  \\ fs [tree_len_eq_def]
+  \\ simp [EL_APPEND]
+  \\ Cases_on `t` \\ fs [tree_balanced_height_def]
+  \\ fs [tree_sfx_list_def]
+  \\ simp [EL_APPEND]
+QED
+
+
+Theorem update_heap_array_eq:
+  tree_list_len_eq xs t ht i ==>
+  (st.heap_array = xs ++ tree_sfx_list t ++ ys) ==>
+  0 < ht ==>
+  (st2 = st with <| heap_array :=
+        xs ++ tree_sfx_list (case t of Node _ l r => Node x l r) ++ ys |>) ==>
+  (update_heap_array i x st = (M_success (), st2))
+Proof
+  simp [fetch "-" "update_heap_array_def"]
+  \\ simp [ml_monadBaseTheory.monad_eqs]
+  \\ rw []
+  \\ imp_res_tac tree_balanced_height_length_sfx_eq
+  \\ simp []
+  \\ fs [tree_list_len_eq_def]
+  \\ Cases_on `t` \\ fs [tree_balanced_height_def]
+  \\ fs [tree_sfx_list_def]
+  \\ simp [LUPDATE_APPEND, LUPDATE_DEF]
+QED
+
+Theorem update_heap_array_eq_intro:
+  tree_list_len_eq xs t ht i ==>
+  (st.heap_array = xs ++ tree_sfx_list t ++ ys) ==>
+  0 < ht ==>
+  (!st' prev_xs. (st = st' with <| heap_array := prev_xs |>) /\
+        (st'.heap_array = xs ++ tree_sfx_list (case t of Node _ l r => Node x l r) ++ ys) ==>
+        (f () st' = (M_success v, st_fin))) ==>
+  (st_ex_bind (update_heap_array i x) f st = (M_success v, st_fin))
+Proof
+  simp [ml_monadBaseTheory.monad_eqs]
+  \\ rw []
+  \\ first_x_assum (irule_at Any)
+  \\ drule_then (irule_at Any) update_heap_array_eq 
+  \\ simp []
+  \\ simp [fetch "-" "state_refs_component_equality"]
+QED
+
+Theorem bind_return_eq:
+  st_ex_bind f return = f
+Proof
+  rw [ml_monadBaseTheory.st_ex_bind_def, ml_monadBaseTheory.st_ex_return_def, FUN_EQ_THM]
+  \\ BasicProvers.EVERY_CASE_TAC \\ simp []
+QED
+
+
+Theorem balanced_sfx_heap_left_eq:
+  tree_balanced_height (ht - 1) l ==>
+  1 < ht ==>
+  (sfx_heap_left (oths + LENGTH (tree_sfx_list l)) ht = oths - 1)
+Proof
+  rw []
+  \\ subgoal `!i. sfx_heap_left i ht = i - (LENGTH (tree_sfx_list l)) - 1`
+  >- (
+    imp_res_tac tree_balanced_height_length_sfx_eq
+    \\ simp [sfx_heap_left_def, SUB_RIGHT_SUB]
+    \\ simp [SUB_RIGHT_ADD]
+  )
+  \\ fs []
+  \\ imp_res_tac (GSYM tree_balanced_height_length_sfx_eq)
+  \\ Cases_on `l` \\ fs [tree_balanced_height_def, tree_sfx_list_def]
+QED
+*)
+
+Definition bs_tree_list_to_list_def:
+  bs_tree_list_to_list ts = FLAT (MAP (\(t, i). bs_tree_to_list i t) (REVERSE ts))
+End
+
+Theorem bs_tree_list_to_list_rec:
+  bs_tree_list_to_list (t_i :: ts) = (
+    bs_tree_list_to_list ts ++ bs_tree_to_list (SND t_i) (FST t_i)
+  ) /\
+  bs_tree_list_to_list [] = []
+Proof
+  simp [bs_tree_list_to_list_def]
+  \\ rpt (pairarg_tac \\ fs[])
+QED
+
+Theorem monad_simps[local] = LIST_CONJ
+    [fetch "-" "update_heap_array_def", fetch "-" "heap_array_sub_def",
+        ml_monadBaseTheory.monad_eqs, st_ex_ignore_bind_simp,
+        fetch "-" "update_sz_array_def", fetch "-" "sz_array_sub_def"]
+
+Theorem tree_len_simps_no_less = LIST_CONJ
+    [tree_balanced_height_def, tree_balanced_height_0,
+        two_exp_min_1_rec,
+        LENGTH_bs_tree_to_list, bs_tree_to_list_def,
+        bs_tree_to_list_tree_rec, bs_tree_list_to_list_rec]
+
+Theorem tree_len_simps = LIST_CONJ [tree_len_simps_no_less,
+        two_exp_min_1_less_rec]
+
+Theorem TAKE_DROP_eq_imp[local]:
+  !xs i j. TAKE i (DROP j xs) = ys ==>
+  i <= LENGTH ys ==>
+  ys = [] \/ (?xs_pre xs_post. xs = xs_pre ++ ys ++ xs_post /\
+    j = LENGTH xs_pre /\ i = LENGTH ys)
+Proof
+  Cases_on `ys = []` \\ simp []
+  \\ rw []
+  \\ qexists_tac `TAKE j xs`
+  \\ qexists_tac `DROP (i + j) xs`
+  \\ fs [GSYM TAKE_SUM]
+  \\ fs [LENGTH_TAKE_EQ]
+QED
+
+Theorem TAKE_DROP_last_eq_imp[local]:
+  TAKE l (DROP ((i + 1) - l) xs) = ys /\
+  i + 1 <= LENGTH xs /\ l <= i + 1 /\
+  l <= LENGTH ys /\ 0 < l ==>
+  ?xs_pre xs_post. xs = xs_pre ++ ys ++ xs_post /\
+    l = LENGTH ys /\ i = LENGTH xs_pre + (LENGTH ys - 1)
+Proof
+  rpt strip_tac
+  \\ dxrule TAKE_DROP_eq_imp
+  \\ Cases_on `ys = []` \\ fs []
+  \\ rw []
+  \\ irule_at Any EQ_REFL
+  \\ simp []
+QED
+
+Theorem insert_into_sfx_heap_eq:
+  ! t R i ht x st.
+  TAKE (two_exp_min_1 ht) (DROP ((i + 1) - two_exp_min_1 ht) st.heap_array) =
+    bs_tree_to_list ht t /\
+  i + 1 <= LENGTH st.heap_array /\
+  two_exp_min_1 ht <= i + 1 /\
+  ht > 0 /\
+  tree_balanced_height ht t ==>
+  (insert_into_sfx_heap R i ht x st =
+  (M_success (), st with <| heap_array := TAKE ((i + 1) - two_exp_min_1 ht) st.heap_array
+    ++ bs_tree_to_list ht (insert_tree_inv R t x) ++ DROP (i + 1) st.heap_array |>))
+Proof
+  Induct
+  \\ simp [tree_len_simps]
+  \\ ONCE_REWRITE_TAC [insert_into_sfx_heap_def]
+  \\ rpt strip_tac
+  \\ dxrule TAKE_DROP_last_eq_imp
+  \\ simp [tree_len_simps]
+  \\ rw [] \\ fs []
+  \\ simp [tree_len_simps, TAKE_APPEND2, TAKE_APPEND1, DROP_APPEND1, DROP_APPEND2]
+  >- (
+    Cases_on `ht = 1` \\ fs [tree_len_simps]
+    \\ fs [insert_tree_inv_def, tree_len_simps]
+    \\ simp [monad_simps, LUPDATE_APPEND, LUPDATE_DEF]
+  )
+  >- (
+    fs [tree_balanced_height_pos]
+    \\ simp [monad_simps, tree_len_simps, sfx_heap_left_two_exp_min_1]
+    \\ simp [EL_APPEND, tree_len_simps, LEFT_ADD_DISTRIB]
+    \\ rpt TOP_CASE_TAC \\ simp [ml_monadBaseTheory.monad_eqs]
+    >- (
+      simp [tree_len_simps, LUPDATE_APPEND, LUPDATE_DEF]
+      \\ simp [insert_tree_inv_def, tree_len_simps]
+    )
+    >- (
+      simp [tree_len_simps, LUPDATE_APPEND, LUPDATE_DEF]
+      \\ ONCE_REWRITE_TAC [insert_tree_inv_def]
+      \\ simp [tree_len_simps]
+      \\ simp [tree_len_simps, TAKE_APPEND2, TAKE_APPEND1, DROP_APPEND1, DROP_APPEND2]
+      \\ simp_tac bool_ss [GSYM APPEND_ASSOC, APPEND]
+    )
+    >- (
+      simp [tree_len_simps, LUPDATE_APPEND, LUPDATE_DEF]
+      \\ ONCE_REWRITE_TAC [insert_tree_inv_def]
+      \\ simp [tree_len_simps]
+      \\ simp [tree_len_simps, TAKE_APPEND2, TAKE_APPEND1, DROP_APPEND1, DROP_APPEND2]
+    )
+  )
+QED
+
+
+Theorem mk_sub_min_1[local]:
+  (x + 1n) - (2 EXP ht) = (x - two_exp_min_1 ht)
+Proof
+  simp [two_exp_min_1_def]
+  \\ Cases_on `2 EXP ht` \\ simp []
+  \\ fs []
+QED
+
+Theorem EL_APPEND_PLUS[local]:
+  EL (LENGTH xs + n) (xs ++ ys) = EL n ys
+Proof
+  simp [EL_APPEND]
+QED
+
+Theorem two_exp_min_1_pos[local]:
+  (0 < two_exp_min_1 r) = (0 < r)
+Proof
+  Cases_on `r` \\ simp [two_exp_min_1_rec]
+QED
+
+Theorem insert_into_sfx_heap_list_eq:
+  ! j ts R i x xs ys st.
+  TAKE (LENGTH (bs_tree_list_to_list ts))
+    (DROP ((i + 1) - (LENGTH (bs_tree_list_to_list ts))) st.heap_array) =
+    bs_tree_list_to_list ts /\
+  i + 1 <= LENGTH st.heap_array /\
+  LENGTH (bs_tree_list_to_list ts) <= i + 1 /\
+  TAKE j st.sz_array = MAP SND (REVERSE ts) /\
+  j <= LENGTH st.sz_array ==>
+  0 < j /\ EVERY (\(t, n). 0 < n /\ tree_balanced_height n t) ts ==>
+  insert_into_sfx_heap_list R i j x st =
+  (M_success (), st with <| heap_array := TAKE ((i + 1) - LENGTH (bs_tree_list_to_list ts)) st.heap_array
+    ++ bs_tree_list_to_list (insert_trees_inv R ts x) ++ DROP (i + 1) st.heap_array |>)
+Proof
+  Induct
+  \\ simp []
+  \\ ONCE_REWRITE_TAC [insert_into_sfx_heap_list_def]
+  \\ rpt strip_tac
+  \\ dxrule TAKE_DROP_last_eq_imp
+  \\ fs [tree_len_simps]
+  \\ Cases_on `HD ts` \\ Cases_on `ts` \\ fs []
+  \\ gs [tree_len_simps]
+  \\ simp [insert_trees_inv_def]
+  \\ rw []
+  >- (
+    Cases_on `t` \\ fs []
+    \\ Cases_on `j` \\ fs []
+    \\ qpat_x_assum `TAKE _ _ = _` (assume_tac o Q.AP_TERM `\x. (EL 0 x, LENGTH x)`)
+    \\ gs [HD_TAKE]
+    \\ simp [monad_simps]
+    \\ drule_at (Pat `tree_balanced_height _ _`) insert_into_sfx_heap_eq
+    \\ simp [tree_len_simps, TAKE_APPEND2, TAKE_APPEND1, DROP_APPEND1, DROP_APPEND2]
+  )
+  >- (
+    gs [tree_len_simps, two_exp_min_1_pos]
+    \\ first_x_assum (qspec_then `t` assume_tac)
+    \\ qpat_x_assum `TAKE _ _ = _` (assume_tac o Q.AP_TERM `\x. (TAKE j x, EL j x, LENGTH x)`)
+    \\ Cases_on `j` \\ fs []
+    \\ Cases_on `HD t` \\ Cases_on `t` \\ fs []
+    \\ gs [ADD1, EL_TAKE, EL_APPEND, TAKE_TAKE]
+    \\ gs [tree_balanced_height_pos]
+    \\ simp [monad_simps, tree_len_simps]
+    \\ full_simp_tac bool_ss [to_two_exp_min_1]
+    \\ full_simp_tac bool_ss [GSYM ADD_ASSOC, GSYM APPEND_ASSOC, EL_APPEND_PLUS]
+    \\ full_simp_tac bool_ss [to_two_exp_min_1]
+    \\ simp [tree_len_simps, TAKE_APPEND2, TAKE_APPEND1, DROP_APPEND1, DROP_APPEND2,
+                EL_APPEND1, EL_APPEND2]
+    \\ TOP_CASE_TAC
+    >- (
+      simp [monad_simps]
+      \\ simp [tree_len_simps, sfx_heap_left_two_exp_min_1, LEFT_ADD_DISTRIB]
+      \\ simp [tree_len_simps, TAKE_APPEND2, TAKE_APPEND1, DROP_APPEND1, DROP_APPEND2,
+                EL_APPEND1, EL_APPEND2]
+      \\ gs [tree_balanced_height_pos]
+      \\ simp [tree_len_simps, TAKE_APPEND2, TAKE_APPEND1, DROP_APPEND1, DROP_APPEND2,
+                EL_APPEND1, EL_APPEND2]
+      \\ rw []
+      >- (
+        simp [monad_simps]
+        \\ simp [tree_len_simps, LUPDATE_APPEND, LUPDATE_DEF]
+        \\ simp [tree_len_simps, TAKE_APPEND2, TAKE_APPEND1, DROP_APPEND1, DROP_APPEND2,
+                EL_APPEND1, EL_APPEND2, LUPDATE_APPEND, LUPDATE_DEF]
+      )
+      >- (
+        irule EQ_TRANS \\ irule_at Any insert_into_sfx_heap_eq
+        \\ simp [tree_len_simps, TAKE_APPEND2, TAKE_APPEND1, DROP_APPEND1, DROP_APPEND2,
+                EL_APPEND1, EL_APPEND2, LUPDATE_APPEND, LUPDATE_DEF]
+        \\ irule_at Any EQ_REFL
+        \\ simp [tree_len_simps]
+      )
+    )
+    >- (
+      simp [monad_simps]
+      \\ simp [tree_len_simps, sfx_heap_left_two_exp_min_1, LEFT_ADD_DISTRIB]
+      \\ TOP_CASE_TAC \\ fs []
+      >- (
+        Cases_on `r = 1` \\ fs []
+        \\ fs [tree_len_simps]
+        \\ simp [monad_simps]
+        \\ fs [tree_len_simps]
+        \\ simp [tree_len_simps, LUPDATE_APPEND, LUPDATE_DEF]
+        \\ simp [tree_len_simps, TAKE_APPEND2, TAKE_APPEND1, DROP_APPEND1, DROP_APPEND2,
+                EL_APPEND1, EL_APPEND2, LUPDATE_APPEND, LUPDATE_DEF]
+        \\ simp_tac bool_ss [GSYM APPEND_ASSOC, APPEND]
+      )
+      >- (
+        irule EQ_TRANS \\ irule_at Any insert_into_sfx_heap_eq
+        \\ simp [tree_len_simps, TAKE_APPEND2, TAKE_APPEND1, DROP_APPEND1, DROP_APPEND2,
+                EL_APPEND1, EL_APPEND2, LUPDATE_APPEND, LUPDATE_DEF]
+        \\ irule_at Any EQ_REFL
+        \\ simp [tree_len_simps]
+      )
+    )
+  )
+QED
+
+Theorem MAP_SND_insert_trees_inv[local]:
+  !ts. MAP SND (insert_trees_inv R ts x) = MAP SND ts
+Proof
+  Induct \\ simp [pairTheory.FORALL_PROD, insert_trees_inv_def]
+  \\ rw []
+  \\ rpt (TOP_CASE_TAC \\ simp [])
+  \\ simp []
+QED
+
+Theorem MAP_LENGTH_insert_trees_inv[local]:
+  MAP (LENGTH o (\(t, n). bs_tree_to_list n t))
+            (insert_trees_inv R ts x) =
+    MAP (LENGTH o (\(t, n). bs_tree_to_list n t)) ts
+Proof
+  qspec_then `ts` (mp_tac o Q.AP_TERM `MAP two_exp_min_1`) MAP_SND_insert_trees_inv
+  \\ simp [MAP_MAP_o, o_DEF, UNCURRY, tree_len_simps]
+QED
+
+Theorem LENGTH_insert_trees_inv[local] =
+  Q.AP_TERM `LENGTH` (SPEC_ALL MAP_LENGTH_insert_trees_inv)
+    |> REWRITE_RULE [LENGTH_MAP]
+
+Theorem LENGTH_list_of_insert_trees[local]:
+  LENGTH (bs_tree_list_to_list (insert_trees_inv R ts x)) =
+  LENGTH (bs_tree_list_to_list ts)
+Proof
+  simp [bs_tree_list_to_list_def, LENGTH_FLAT, MAP_MAP_o, MAP_REVERSE]
+  \\ simp [MAP_LENGTH_insert_trees_inv]
+QED
+
+Theorem TAKE_EQ_GENLIST:
+  !n xs. TAKE n xs = GENLIST (\i. EL i xs) (MIN n (LENGTH xs))
+Proof
+  Induct \\ rw []
+  \\ Cases_on `xs` \\ fs []
+  \\ irule EQ_SYM
+  \\ simp [llistTheory.GENLIST_EQ_CONS]
+  \\ simp [o_DEF, MIN_DEF]
+  \\ rw []
+QED
+
+Theorem bind_assoc:
+  st_ex_bind (st_ex_bind f g) h = do
+    x <- f;
+    y <- g x;
+    h y
+  od
+Proof
+  rw [ml_monadBaseTheory.st_ex_bind_def, FUN_EQ_THM]
+  \\ rpt (TOP_CASE_TAC \\ fs [])
+QED
+
+Theorem add_to_sfx_heaps_step1_eq:
+  EVERY (\(t, n). 0 < n /\ tree_balanced_height n t) ts ==>
+  TAKE i st.heap_array = bs_tree_list_to_list ts /\
+  TAKE j st.sz_array = MAP SND (REVERSE ts) /\
+  j = LENGTH ts /\ i = LENGTH (bs_tree_list_to_list ts) /\
+  i + 1 < LENGTH st.heap_array /\
+  j + 1 < LENGTH st.sz_array ==>
+  ?st'.
+  (let ts2 = add_trees_step1 ts (EL i st.heap_array);
+        xs = bs_tree_list_to_list ts2; l2 = LENGTH ts2 in
+  add_to_sfx_heaps_step1 i j st = (M_success l2, st') /\
+  TAKE (i + 1) st'.heap_array = xs /\
+  TAKE l2 st'.sz_array = MAP SND (REVERSE ts2) /\
+  LENGTH st'.sz_array = LENGTH st.sz_array /\
+  LENGTH st'.heap_array = LENGTH st.heap_array
+  )
+Proof
+  rw []
+  \\ simp [add_to_sfx_heaps_step1_def, add_trees_step1_def]
+  \\ Cases_on `ts` \\ fs []
+  >- (
+    simp [monad_simps]
+    \\ fs [tree_len_simps]
+    \\ fs [Q.SPEC `1` TAKE_EQ_GENLIST, MIN_DEF, EL_LUPDATE, HD_LUPDATE]
+  )
+  \\ Cases_on `t` \\ fs []
+  >- (
+    simp [monad_simps]
+    \\ fs [tree_len_simps]
+    \\ fs [Q.SPEC `2` TAKE_EQ_GENLIST, Q.SPEC `1` TAKE_EQ_GENLIST, MIN_DEF, EL_LUPDATE, HD_LUPDATE]
+    \\ fs [TAKE_SUM]
+  )
+  \\ rpt (TOP_CASE_TAC \\ fs [])
+  >- (
+    simp [monad_simps]
+    \\ fs [ADD1, TAKE_SUM, EL_DROP, EL_LUPDATE]
+    \\ gs [Q.SPEC `2` TAKE_EQ_GENLIST, Q.SPEC `1` TAKE_EQ_GENLIST, MIN_DEF, HD_DROP, EL_DROP]
+    \\ simp [monad_simps]
+    \\ fs [tree_len_simps_no_less, HD_DROP, EL_LUPDATE]
+    \\ irule EQ_TRANS
+    \\ first_x_assum (irule_at Any)
+    \\ irule listTheory.LIST_EQ
+    \\ simp [EL_TAKE, EL_LUPDATE]
+  )
+  >- (
+    simp [monad_simps]
+    \\ fs [ADD1, TAKE_SUM, EL_DROP, EL_LUPDATE]
+    \\ gs [Q.SPEC `2` TAKE_EQ_GENLIST, Q.SPEC `1` TAKE_EQ_GENLIST, MIN_DEF, HD_DROP, EL_DROP]
+    \\ simp [monad_simps]
+    \\ fs [tree_len_simps_no_less, HD_DROP, EL_LUPDATE]
+    \\ qpat_x_assum `_ = MAP _ (REVERSE _)` (assume_tac o GSYM)
+    \\ irule listTheory.LIST_EQ
+    \\ rw [EL_TAKE, EL_APPEND]
+    \\ simp [EL_LUPDATE, EL_DROP]
+    \\ rw []
+    \\ Cases_on `x = LENGTH t'` \\ fs []
+    \\ Cases_on `x = LENGTH t' + 1` \\ fs []
+  )
+QED
+
+Theorem LENGTH_add_trees_step1_adj[local]:
+  LENGTH (add_trees_step1 ts x) = LENGTH (I (add_trees_step1 ts) ARB)
+Proof
+  simp [add_trees_step1_def]
+  \\ rpt (TOP_CASE_TAC \\ fs [])
+QED
+
+Theorem LENGTH_add_tree_step1_facts:
+  0 < LENGTH (add_trees_step1 ts x) /\
+  LENGTH (bs_tree_list_to_list (add_trees_step1 ts x)) =
+    LENGTH (bs_tree_list_to_list ts) + 1 /\
+  LENGTH (add_trees_step1 ts x) <= LENGTH ts + 1 /\
+  (MAP SND (add_trees_step1 ts x) = MAP SND (add_trees_step1 ts y)) = T /\
+  (LENGTH (add_trees_step1 ts x) = LENGTH (add_trees_step1 ts y)) = T
+Proof
+  simp [add_trees_step1_def]
+  \\ rpt (TOP_CASE_TAC \\ fs [tree_len_simps])
+QED
+
+Theorem inv_add_tree_step1:
+  (EVERY (\(t,n). 0 < n /\ tree_balanced_height n t) ts ==>
+    EVERY (\(t,n). 0 < n /\ tree_balanced_height n t) (add_trees_step1 ts x)
+  ) /\
+  (EVERY (\(t,n). 0 < n /\ tree_balanced_height n t) ts /\
+    SORTED ($<=) (TAKE 2 (MAP SND ts)) /\ SORTED ($<) (MAP SND (DROP 1 ts)) ==>
+    SORTED ($<=) (TAKE 2 (MAP SND (add_trees_step1 ts x))) /\
+    SORTED ($<) (MAP SND (DROP 1 (add_trees_step1 ts x)))
+  )
+Proof
+  simp [add_trees_step1_def]
+  \\ rpt (TOP_CASE_TAC \\ fs [tree_len_simps])
+  \\ rpt (pairarg_tac \\ fs [])
+  \\ rw []
+  \\ fs []
+  \\ imp_res_tac SORTED_TL \\ fs []
+  \\ Cases_on `t'` \\ fs []
+QED
+
+Theorem insert_trees_adj_with_inv[local]:
+  EVERY (\(t,n). 0 < n /\ tree_balanced_height n t) ts ==>
+  insert_trees_inv R ((Node x_dc l r, n) :: ts) x =
+      insert_trees_inv R ((Node y_dc l r, n) :: ts) x
+Proof
+  simp [insert_trees_inv_def]
+  \\ rpt (TOP_CASE_TAC \\ fs []) \\ rw [] \\ fs [tree_len_simps]
+  \\ simp [insert_tree_inv_def]
+QED
+
+Theorem insert_trees_adj_add_trees_with_inv[local]:
+  EVERY (\(t,n). 0 < n /\ tree_balanced_height n t) ts ==>
+  insert_trees_inv R (add_trees_step1 ts x_dc) x =
+      insert_trees_inv R (add_trees_step1 ts y_dc) x
+Proof
+  simp [add_trees_step1_def]
+  \\ rpt (TOP_CASE_TAC \\ fs [tree_len_simps])
+  \\ rw []
+  \\ irule insert_trees_adj_with_inv
+  \\ simp []
+QED
+
+Theorem add_to_sfx_heaps_eq:
+  EVERY (\(t, n). 0 < n /\ tree_balanced_height n t) ts ==>
+  TAKE i st.heap_array = bs_tree_list_to_list ts /\
+  TAKE j st.sz_array = MAP SND (REVERSE ts) /\
+  j = LENGTH ts /\ i = LENGTH (bs_tree_list_to_list ts) /\
+  i + 1 < LENGTH st.heap_array /\
+  j + 1 < LENGTH st.sz_array ==>
+  ?st'.
+  (let ts2 = add_trees R ts x; xs = bs_tree_list_to_list ts2; l2 = LENGTH ts2 in
+  add_to_sfx_heaps R i j x st = (M_success l2, st') /\
+  TAKE (i + 1) st'.heap_array = xs /\
+  TAKE l2 st'.sz_array = MAP SND (REVERSE ts2) /\
+  LENGTH st'.sz_array = LENGTH st.sz_array /\
+  LENGTH st'.heap_array = LENGTH st.heap_array
+  )
+Proof
+  simp [add_to_sfx_heaps_def, add_trees_def]
+  \\ rpt strip_tac
+  \\ mp_tac add_to_sfx_heaps_step1_eq
+  \\ rpt strip_tac
+  \\ gs [monad_simps]
+  \\ irule_at Any insert_into_sfx_heap_list_eq
+  \\ qexists_tac `add_trees_step1 ts (EL i st.heap_array)`
+  \\ fs [tree_len_simps_no_less, LENGTH_insert_trees_inv]
+  \\ fs [LENGTH_add_tree_step1_facts, inv_add_tree_step1, LENGTH_list_of_insert_trees]
+  \\ rpt conj_tac
+  >- (
+    irule LESS_EQ_TRANS
+    \\ MAP_FIRST (irule_at Any) (CONJUNCTS LENGTH_add_tree_step1_facts)
+    \\ simp []
+  )
+  >- (
+    simp [TAKE_APPEND1, LENGTH_add_tree_step1_facts, LENGTH_list_of_insert_trees,
+        TAKE_LENGTH_TOO_LONG]
+    \\ AP_TERM_TAC
+    \\ irule insert_trees_adj_add_trees_with_inv
+    \\ simp []
+  )
+  >- (
+    simp [MAP_REVERSE, MAP_SND_insert_trees_inv]
+    \\ irule (Q.prove (`a = b /\ TAKE b xs = zs/\ zs = ys ==> TAKE a xs = ys`, simp []))
+    \\ first_x_assum (irule_at Any)
+    \\ simp [MAP_REVERSE, LENGTH_add_tree_step1_facts]
+  )
+QED
+
+Theorem LENGTH_to_list_add_trees:
+  LENGTH (bs_tree_list_to_list (add_trees R ts x)) = 
+    LENGTH (bs_tree_list_to_list ts) + 1
+Proof
+  simp [add_trees_def, LENGTH_list_of_insert_trees, LENGTH_add_tree_step1_facts]
+QED
+
+Theorem insert_tree_inv_balance_inv:
+  !t ht. tree_balanced_height ht t ==>
+  tree_balanced_height ht (insert_tree_inv R t x)
+Proof
+  Induct \\ simp [insert_tree_inv_def]
+  \\ rpt (TOP_CASE_TAC \\ fs [tree_len_simps])
+QED
+
+Theorem insert_trees_inv_balance_inv:
+  !ts x. EVERY (\(t,n). 0 < n /\ tree_balanced_height n t) ts ==>
+  EVERY (\(t,n). 0 < n /\ tree_balanced_height n t) (insert_trees_inv R ts x)
+Proof
+  Induct \\ simp [pairTheory.FORALL_PROD, insert_trees_inv_def]
+  \\ rw []
+  \\ rpt (TOP_CASE_TAC \\ fs [tree_len_simps, insert_tree_inv_balance_inv])
+QED
+
+Theorem inv_add_tree:
+  (EVERY (\(t,n). 0 < n /\ tree_balanced_height n t) ts ==>
+    EVERY (\(t,n). 0 < n /\ tree_balanced_height n t) (add_trees R ts x)
+  ) /\
+  (EVERY (\(t,n). 0 < n /\ tree_balanced_height n t) ts /\
+    SORTED ($<=) (TAKE 2 (MAP SND ts)) /\ SORTED ($<) (MAP SND (DROP 1 ts)) ==>
+    SORTED ($<=) (TAKE 2 (MAP SND (add_trees R ts x))) /\
+    SORTED ($<) (MAP SND (DROP 1 (add_trees R ts x)))
+  )
+Proof
+  simp [add_trees_def, MAP_SND_insert_trees_inv, MAP_DROP]
+  \\ simp [GSYM MAP_DROP, inv_add_tree_step1, insert_trees_inv_balance_inv]
+QED
+
+Theorem sum_gt_exp_2:
+  !js n. EVERYi (\i j. j >= (2 EXP i) * n) js ==>
+  SUM js >= ((2 EXP LENGTH js) - 1) * n
+Proof
+  Induct
+  \\ rw [EVERYi_def]
+  \\ first_x_assum (qspec_then `2 * n` mp_tac)
+  \\ fs [o_DEF, EXP]
+QED
+
+Theorem sum_lengths_greater_equal_exp[local]:
+  ! ts n. EVERY (\(t,n). 0 < n /\ tree_balanced_height n t) ts /\
+  SORTED $< (MAP SND ts) /\
+  ts <> [] /\ n <= SND (HD ts) /\ 1 <= n ==>
+  ((2 EXP (LENGTH ts + (n - 1))) - 1) <= LENGTH (bs_tree_list_to_list ts)
+Proof
+  Induct \\ rw []
+  \\ fs [tree_len_simps]
+  \\ pairarg_tac \\ fs []
+  \\ first_x_assum (qspec_then `SUC n` mp_tac)
+  \\ imp_res_tac SORTED_TL
+  \\ simp [tree_len_simps, EXP]
+  \\ Cases_on `ts` \\ fs []
+  >- (
+    simp [tree_len_simps]
+    \\ simp [two_exp_min_1_def, LEFT_SUB_DISTRIB]
+    \\ simp [GSYM EXP, ADD1]
+    \\ rw [SUB_RIGHT_ADD]
+  )
+  >- (
+    rw []
+    \\ gs [ADD1]
+  )
+QED
+
+Theorem inv_trees_less_via_exp[local]:
+  EVERY (\(t,n). 0 < n /\ tree_balanced_height n t) ts /\
+  SORTED $< (DROP 1 (MAP SND ts)) /\
+  LENGTH (bs_tree_list_to_list ts) < 2 ** lg /\
+  lg + i + 2 <= bd ==>
+  LENGTH ts + i < bd
+Proof
+  rw []
+  \\ fs [GSYM MAP_DROP]
+  \\ drule_at (Pat `SORTED _ _`) sum_lengths_greater_equal_exp
+  \\ simp [EVERY_DROP]
+  \\ disch_then (qspec_then `1` mp_tac)
+  \\ Cases_on `LENGTH ts <= 1` \\ fs []
+  \\ impl_tac
+  >- (
+    fs [HD_DROP, EVERY_EL, UNCURRY]
+    \\ first_x_assum (qspec_then `1` mp_tac)
+    \\ simp []
+  )
+  \\ disch_tac
+  \\ subgoal `2n ** (LENGTH ts - 1) < 2 ** lg`
+  >- (
+    drule_then irule LESS_EQ_LESS_TRANS
+    \\ Cases_on `ts` \\ fs [tree_len_simps]
+    \\ pairarg_tac \\ fs []
+    \\ gs [tree_len_simps]
+  )
+  \\ fs []
+QED
+
+Theorem add_all_to_sfx_heaps_eq:
+  !xs i j ts st. EVERY (\(t, n). 0 < n /\ tree_balanced_height n t) ts /\
+  SORTED ($<=) (TAKE 2 (MAP SND ts)) /\ SORTED ($<) (MAP SND (DROP 1 ts)) /\
+  TAKE i st.heap_array = bs_tree_list_to_list ts /\
+  TAKE j st.sz_array = MAP SND (REVERSE ts) /\
+  j = LENGTH ts /\ i = LENGTH (bs_tree_list_to_list ts) /\
+  i + LENGTH xs < LENGTH st.heap_array /\
+  lg + 3 <= LENGTH st.sz_array /\
+  i + LENGTH xs < 2 EXP lg ==>
+  ?st'.
+  (let ts2 = build_trees R ts xs; ys = bs_tree_list_to_list ts2; l2 = LENGTH ts2 in
+  add_all_to_sfx_heaps R i j xs st = (M_success (LENGTH ys, l2), st') /\
+  TAKE (LENGTH ys) st'.heap_array = ys /\
+  TAKE l2 st'.sz_array = MAP SND (REVERSE ts2) /\
+  LENGTH st'.sz_array = LENGTH st.sz_array /\
+  LENGTH st'.heap_array = LENGTH st.heap_array
+  )
+Proof
+  Induct
+  \\ rw [add_all_to_sfx_heaps_def, build_trees_def]
+  \\ simp [monad_simps]
+  \\ fs []
+  \\ qmatch_goalsub_abbrev_tac `add_to_sfx_heaps _ i j  x`
+  \\ mp_tac add_to_sfx_heaps_eq
+  \\ simp []
+  \\ impl_tac
+  >- (
+    fs [markerTheory.Abbrev_def]
+    \\ irule inv_trees_less_via_exp
+    \\ simp [GSYM MAP_DROP]
+    \\ qexists_tac `lg` \\ simp []
+  )
+  \\ rw []
+  \\ last_x_assum (drule_at (Pat `_ = MAP _ _`))
+  \\ gs [markerTheory.Abbrev_def, LENGTH_to_list_add_trees]
+  \\ simp [inv_add_tree]
+QED
+
+(* TODO: reinsert tree, sfx_trees_to_list and toplevel
+
+Theorem reinsert_tree_eq:
+
+  EVERY (\(t, n). 0 < n /\ tree_balanced_height n t) ts /\
+  SORTED ($<=) (TAKE 2 (MAP SND ts)) /\ SORTED ($<) (MAP SND (DROP 1 ts)) /\
+  TAKE i st.heap_array = bs_tree_list_to_list ts ++ bs_tree_to_list ht t /\
+  TAKE j st.sz_array = MAP SND (REVERSE ts) /\
+  j = LENGTH ts /\ i = LENGTH (bs_tree_list_to_list ts ++ bs_tree_to_list ht t) /\
+  i + LENGTH xs < LENGTH st.heap_array /\
+  lg + 3 <= LENGTH st.sz_array /\
+  i + LENGTH xs < 2 EXP lg /\
+  0 < ht /\ tree_balanced_height ht t ==>
+  ?st'.
+  (let ts2 = extend_trees R ts t ht; ys = bs_tree_list_to_list ts2; l2 = LENGTH ts2 in
+  reinsert_tree R i j ht st = (M_success (), st') /\
+  TAKE (LENGTH ys) st'.heap_array = ys /\
+  DROP (LENGTH ys) st'.heap_array = DROP (LENGTH ys) st.heap_array /\
+  TAKE l2 st'.sz_array = MAP SND (REVERSE ts2) /\
+  LENGTH st'.sz_array = LENGTH st.sz_array /\
+  LENGTH st'.heap_array = LENGTH st.heap_array
+  )
+
+Proof
+
+  rw [reinsert_tree_def]
+  \\ simp [monad_simps]
+  \\ drule inv_trees_less_via_exp
+  \\ simp [GSYM MAP_DROP]
+  \\ disch_then (qspecl_then [`lg`, `0`, `LENGTH st.sz_array`] mp_tac)
+  \\ rw []
+
+  >- (
+    simp [monad_simps]
+    \\ gs [tree_len_simps, to_two_exp_min_1, tree_balanced_height_pos]
+    \\ fs [TAKE_SUM, EL_DROP]
+    \\ Cases_on `ts` \\ fs []
+    \\ pairarg_tac \\ fs []
+    \\ gs [tree_len_simps, tree_balanced_height_pos]
+    \\ fs [TAKE_SUM, EL_DROP]
+    \\ fs [listTheory.APPEND_11_LENGTH, LENGTH_TAKE, LENGTH_DROP]
+
+
+print_match [] ``(_ ++ _) = (_ ++ _)``
+
+ 
+
+Theorem sfx_trees_to_list_eq:
+
+  !i j acc ts st. EVERY (\(t, n). 0 < n /\ tree_balanced_height n t) ts /\
+  SORTED ($<=) (TAKE 2 (MAP SND ts)) /\ SORTED ($<) (MAP SND (DROP 1 ts)) /\
+  TAKE i st.heap_array = bs_tree_list_to_list ts /\
+  TAKE j st.sz_array = MAP SND (REVERSE ts) /\
+  j = LENGTH ts /\ i = LENGTH (bs_tree_list_to_list ts) /\
+  i < LENGTH st.heap_array /\
+  lg + 4 <= LENGTH st.sz_array /\
+  i < 2 EXP lg ==>
+  ?st'. sfx_trees_to_list R i j acc st = (M_success (pull_trees R ts acc), st')
+
+Proof
+
+  Induct
+  \\ ONCE_REWRITE_TAC [sfx_trees_to_list_def]
+  >- (
+    rw []
+    \\ Cases_on `ts` \\ fs []
+    \\ simp [monad_simps, pull_trees_def]
+    \\ rpt (pairarg_tac \\ fs []) \\ gs [tree_len_simps, tree_balanced_height_pos]
+  )
+  \\ rw []
+  \\ simp [monad_simps]
+  \\ drule inv_trees_less_via_exp
+  \\ simp [GSYM MAP_DROP]
+  \\ disch_then (qspecl_then [`lg`, `0`, `LENGTH st.sz_array`] mp_tac)
+  \\ rw []
+  >- (
+    Cases_on `ts` \\ fs [tree_len_simps]
+    \\ pairarg_tac \\ fs []
+    \\ gs [tree_len_simps, tree_balanced_height_pos]
+    \\ gs [ADD1, TAKE_SUM]
+    \\ Cases_on `n = 1` \\ fs [tree_len_simps]
+    \\ simp [pull_trees_def, extend_trees_def]
+    \\ fs [HD_DROP]
+    \\ first_x_assum irule
+    \\ simp []
+    \\ Cases_on `t` \\ fs []
+    \\ imp_res_tac SORTED_TL
+    \\ simp []
+    \\ qmatch_goalsub_abbrev_tac `TAKE 1 tl_ts`
+    \\ Cases_on `tl_ts` \\ fs []
+  )
+  >- (
+    simp [monad_simps, sfx_heap_left_two_exp_min_1]
+    \\ Cases_on `ts` \\ fs [tree_len_simps]
+    \\ pairarg_tac \\ fs []
+    \\ gs [tree_len_simps, tree_balanced_height_pos]
+    \\ gs [ADD1, TAKE_SUM]
+    \\ fs [tree_len_simps, LEFT_ADD_DISTRIB]
+    \\ irule_at Any (Q.SPECL [`j`, `(t, n) :: ts`] insert_into_sfx_heap_list_eq)
+    \\ simp [ADD1, TAKE_SUM, EL_LUPDATE]
+    \\ simp [tree_len_simps]
+    \\ qexists_tac `t` \\ simp []
+    \\ hphp
+
+
+TAKE1
+
+  \\,  rpt (pairarg_tac \\ fs []) \\ gs [tree_len_simps, tree_balanced_height_pos]
+  \\ fs [ADD1]
+  \\ 
+
+    \\ irule inv_trees_less_via_exp
+*)
 
